proofs/talos/lean/Project/EulerOutwardMaximum/ArtifactTranslation.lean
@@ -1,0 +1,356 @@
+import Project.EulerOutwardMaximum.ArtifactValidation
+import Project.EulerOutwardMaximum.Spec
+import Project.EulerOutwardMaximum.Program
+import Project.Artifact.Binary.Proof.Translate
+import Project.Artifact.Binary.Proof.Validate
+
+set_option maxRecDepth 1048576
+
+namespace Project.EulerOutwardMaximum.Artifact
+
+open Wasm
+open Wasm.Binary
+
+theorem function0_eq :
+    Translation.functionToTalos Cache.raw 0 (Cache.raw.codes[0]!) =
+      Project.EulerOutwardMaximum.func0Def := by
+  rfl
+
+theorem function1_eq :
+    Translation.functionToTalos Cache.raw 1 (Cache.raw.codes[1]!) =
+      Project.EulerOutwardMaximum.func1Def := by
+  rfl
+
+theorem function2_eq :
+    Translation.functionToTalos Cache.raw 2 (Cache.raw.codes[2]!) =
+      Project.EulerOutwardMaximum.func2Def := by
+  rfl
+
+theorem function3_eq :
+    Translation.functionToTalos Cache.raw 3 (Cache.raw.codes[3]!) =
+      Project.EulerOutwardMaximum.func3Def := by
+  rfl
+
+theorem function4_eq :
+    Translation.functionToTalos Cache.raw 4 (Cache.raw.codes[4]!) =
+      Project.EulerOutwardMaximum.func4Def := by
+  rfl
+
+theorem function5_eq :
+    Translation.functionToTalos Cache.raw 5 (Cache.raw.codes[5]!) =
+      Project.EulerOutwardMaximum.func5Def := by
+  rfl
+
+theorem function6_eq :
+    Translation.functionToTalos Cache.raw 6 (Cache.raw.codes[6]!) =
+      Project.EulerOutwardMaximum.func6Def := by
+  rfl
+
+theorem function7_eq :
+    Translation.functionToTalos Cache.raw 7 (Cache.raw.codes[7]!) =
+      Project.EulerOutwardMaximum.func7Def := by
+  rfl
+
+theorem function8_eq :
+    Translation.functionToTalos Cache.raw 8 (Cache.raw.codes[8]!) =
+      Project.EulerOutwardMaximum.func8Def := by
+  rfl
+
+theorem function9_eq :
+    Translation.functionToTalos Cache.raw 9 (Cache.raw.codes[9]!) =
+      Project.EulerOutwardMaximum.func9Def := by
+  rfl
+
+theorem function10_eq :
+    Translation.functionToTalos Cache.raw 10 (Cache.raw.codes[10]!) =
+      Project.EulerOutwardMaximum.func10Def := by
+  rfl
+
+theorem function11_eq :
+    Translation.functionToTalos Cache.raw 11 (Cache.raw.codes[11]!) =
+      Project.EulerOutwardMaximum.func11Def := by
+  rfl
+
+theorem function12_eq :
+    Translation.functionToTalos Cache.raw 12 (Cache.raw.codes[12]!) =
+      Project.EulerOutwardMaximum.func12Def := by
+  rfl
+
+theorem function13_eq :
+    Translation.functionToTalos Cache.raw 13 (Cache.raw.codes[13]!) =
+      Project.EulerOutwardMaximum.func13Def := by
+  rfl
+
+theorem function14_eq :
+    Translation.functionToTalos Cache.raw 14 (Cache.raw.codes[14]!) =
+      Project.EulerOutwardMaximum.func14Def := by
+  rfl
+
+theorem function15_eq :
+    Translation.functionToTalos Cache.raw 15 (Cache.raw.codes[15]!) =
+      Project.EulerOutwardMaximum.func15Def := by
+  rfl
+
+theorem function16_eq :
+    Translation.functionToTalos Cache.raw 16 (Cache.raw.codes[16]!) =
+      Project.EulerOutwardMaximum.func16Def := by
+  rfl
+
+theorem function17_eq :
+    Translation.functionToTalos Cache.raw 17 (Cache.raw.codes[17]!) =
+      Project.EulerOutwardMaximum.func17Def := by
+  rfl
+
+theorem function18_eq :
+    Translation.functionToTalos Cache.raw 18 (Cache.raw.codes[18]!) =
+      Project.EulerOutwardMaximum.func18Def := by
+  rfl
+
+theorem function19_eq :
+    Translation.functionToTalos Cache.raw 19 (Cache.raw.codes[19]!) =
+      Project.EulerOutwardMaximum.func19Def := by
+  rfl
+
+theorem function20_eq :
+    Translation.functionToTalos Cache.raw 20 (Cache.raw.codes[20]!) =
+      Project.EulerOutwardMaximum.func20Def := by
+  rfl
+
+theorem function21_eq :
+    Translation.functionToTalos Cache.raw 21 (Cache.raw.codes[21]!) =
+      Project.EulerOutwardMaximum.func21Def := by
+  rfl
+
+theorem function22_eq :
+    Translation.functionToTalos Cache.raw 22 (Cache.raw.codes[22]!) =
+      Project.EulerOutwardMaximum.func22Def := by
+  rfl
+
+theorem function23_eq :
+    Translation.functionToTalos Cache.raw 23 (Cache.raw.codes[23]!) =
+      Project.EulerOutwardMaximum.func23Def := by
+  rfl
+
+theorem function24_eq :
+    Translation.functionToTalos Cache.raw 24 (Cache.raw.codes[24]!) =
+      Project.EulerOutwardMaximum.func24Def := by
+  rfl
+
+theorem function25_eq :
+    Translation.functionToTalos Cache.raw 25 (Cache.raw.codes[25]!) =
+      Project.EulerOutwardMaximum.func25Def := by
+  rfl
+
+theorem function26_eq :
+    Translation.functionToTalos Cache.raw 26 (Cache.raw.codes[26]!) =
+      Project.EulerOutwardMaximum.func26Def := by
+  rfl
+
+theorem function27_eq :
+    Translation.functionToTalos Cache.raw 27 (Cache.raw.codes[27]!) =
+      Project.EulerOutwardMaximum.func27Def := by
+  rfl
+
+theorem function28_eq :
+    Translation.functionToTalos Cache.raw 28 (Cache.raw.codes[28]!) =
+      Project.EulerOutwardMaximum.func28Def := by
+  rfl
+
+theorem function29_eq :
+    Translation.functionToTalos Cache.raw 29 (Cache.raw.codes[29]!) =
+      Project.EulerOutwardMaximum.func29Def := by
+  rfl
+
+theorem function30_eq :
+    Translation.functionToTalos Cache.raw 30 (Cache.raw.codes[30]!) =
+      Project.EulerOutwardMaximum.func30Def := by
+  rfl
+
+theorem function31_eq :
+    Translation.functionToTalos Cache.raw 31 (Cache.raw.codes[31]!) =
+      Project.EulerOutwardMaximum.func31Def := by
+  rfl
+
+theorem function32_eq :
+    Translation.functionToTalos Cache.raw 32 (Cache.raw.codes[32]!) =
+      Project.EulerOutwardMaximum.func32Def := by
+  rfl
+
+theorem function33_eq :
+    Translation.functionToTalos Cache.raw 33 (Cache.raw.codes[33]!) =
+      Project.EulerOutwardMaximum.func33Def := by
+  rfl
+
+theorem function34_eq :
+    Translation.functionToTalos Cache.raw 34 (Cache.raw.codes[34]!) =
+      Project.EulerOutwardMaximum.func34Def := by
+  rfl
+
+theorem function35_eq :
+    Translation.functionToTalos Cache.raw 35 (Cache.raw.codes[35]!) =
+      Project.EulerOutwardMaximum.func35Def := by
+  rfl
+
+theorem function36_eq :
+    Translation.functionToTalos Cache.raw 36 (Cache.raw.codes[36]!) =
+      Project.EulerOutwardMaximum.func36Def := by
+  rfl
+
+theorem function37_eq :
+    Translation.functionToTalos Cache.raw 37 (Cache.raw.codes[37]!) =
+      Project.EulerOutwardMaximum.func37Def := by
+  rfl
+
+theorem function38_eq :
+    Translation.functionToTalos Cache.raw 38 (Cache.raw.codes[38]!) =
+      Project.EulerOutwardMaximum.func38Def := by
+  rfl
+
+theorem function39_eq :
+    Translation.functionToTalos Cache.raw 39 (Cache.raw.codes[39]!) =
+      Project.EulerOutwardMaximum.func39Def := by
+  rfl
+
+theorem function40_eq :
+    Translation.functionToTalos Cache.raw 40 (Cache.raw.codes[40]!) =
+      Project.EulerOutwardMaximum.func40Def := by
+  rfl
+
+theorem function41_eq :
+    Translation.functionToTalos Cache.raw 41 (Cache.raw.codes[41]!) =
+      Project.EulerOutwardMaximum.func41Def := by
+  rfl
+
+theorem function42_eq :
+    Translation.functionToTalos Cache.raw 42 (Cache.raw.codes[42]!) =
+      Project.EulerOutwardMaximum.func42Def := by
+  rfl
+
+theorem function43_eq :
+    Translation.functionToTalos Cache.raw 43 (Cache.raw.codes[43]!) =
+      Project.EulerOutwardMaximum.func43Def := by
+  rfl
+
+theorem function44_eq :
+    Translation.functionToTalos Cache.raw 44 (Cache.raw.codes[44]!) =
+      Project.EulerOutwardMaximum.func44Def := by
+  rfl
+
+theorem function45_eq :
+    Translation.functionToTalos Cache.raw 45 (Cache.raw.codes[45]!) =
+      Project.EulerOutwardMaximum.func45Def := by
+  rfl
+
+theorem function46_eq :
+    Translation.functionToTalos Cache.raw 46 (Cache.raw.codes[46]!) =
+      Project.EulerOutwardMaximum.func46Def := by
+  rfl
+
+theorem functions_eq : Translation.functions Cache.raw =
+    Project.EulerOutwardMaximum.«module».funcs := by
+  change
+    [
+     Translation.functionToTalos Cache.raw 0 (Cache.raw.codes[0]!),
+     Translation.functionToTalos Cache.raw 1 (Cache.raw.codes[1]!),
+     Translation.functionToTalos Cache.raw 2 (Cache.raw.codes[2]!),
+     Translation.functionToTalos Cache.raw 3 (Cache.raw.codes[3]!),
+     Translation.functionToTalos Cache.raw 4 (Cache.raw.codes[4]!),
+     Translation.functionToTalos Cache.raw 5 (Cache.raw.codes[5]!),
+     Translation.functionToTalos Cache.raw 6 (Cache.raw.codes[6]!),
+     Translation.functionToTalos Cache.raw 7 (Cache.raw.codes[7]!),
+     Translation.functionToTalos Cache.raw 8 (Cache.raw.codes[8]!),
+     Translation.functionToTalos Cache.raw 9 (Cache.raw.codes[9]!),
+     Translation.functionToTalos Cache.raw 10 (Cache.raw.codes[10]!),
+     Translation.functionToTalos Cache.raw 11 (Cache.raw.codes[11]!),
+     Translation.functionToTalos Cache.raw 12 (Cache.raw.codes[12]!),
+     Translation.functionToTalos Cache.raw 13 (Cache.raw.codes[13]!),
+     Translation.functionToTalos Cache.raw 14 (Cache.raw.codes[14]!),
+     Translation.functionToTalos Cache.raw 15 (Cache.raw.codes[15]!),
+     Translation.functionToTalos Cache.raw 16 (Cache.raw.codes[16]!),
+     Translation.functionToTalos Cache.raw 17 (Cache.raw.codes[17]!),
+     Translation.functionToTalos Cache.raw 18 (Cache.raw.codes[18]!),
+     Translation.functionToTalos Cache.raw 19 (Cache.raw.codes[19]!),
+     Translation.functionToTalos Cache.raw 20 (Cache.raw.codes[20]!),
+     Translation.functionToTalos Cache.raw 21 (Cache.raw.codes[21]!),
+     Translation.functionToTalos Cache.raw 22 (Cache.raw.codes[22]!),
+     Translation.functionToTalos Cache.raw 23 (Cache.raw.codes[23]!),
+     Translation.functionToTalos Cache.raw 24 (Cache.raw.codes[24]!),
+     Translation.functionToTalos Cache.raw 25 (Cache.raw.codes[25]!),
+     Translation.functionToTalos Cache.raw 26 (Cache.raw.codes[26]!),
+     Translation.functionToTalos Cache.raw 27 (Cache.raw.codes[27]!),
+     Translation.functionToTalos Cache.raw 28 (Cache.raw.codes[28]!),
+     Translation.functionToTalos Cache.raw 29 (Cache.raw.codes[29]!),
+     Translation.functionToTalos Cache.raw 30 (Cache.raw.codes[30]!),
+     Translation.functionToTalos Cache.raw 31 (Cache.raw.codes[31]!),
+     Translation.functionToTalos Cache.raw 32 (Cache.raw.codes[32]!),
+     Translation.functionToTalos Cache.raw 33 (Cache.raw.codes[33]!),
+     Translation.functionToTalos Cache.raw 34 (Cache.raw.codes[34]!),
+     Translation.functionToTalos Cache.raw 35 (Cache.raw.codes[35]!),
+     Translation.functionToTalos Cache.raw 36 (Cache.raw.codes[36]!),
+     Translation.functionToTalos Cache.raw 37 (Cache.raw.codes[37]!),
+     Translation.functionToTalos Cache.raw 38 (Cache.raw.codes[38]!),
+     Translation.functionToTalos Cache.raw 39 (Cache.raw.codes[39]!),
+     Translation.functionToTalos Cache.raw 40 (Cache.raw.codes[40]!),
+     Translation.functionToTalos Cache.raw 41 (Cache.raw.codes[41]!),
+     Translation.functionToTalos Cache.raw 42 (Cache.raw.codes[42]!),
+     Translation.functionToTalos Cache.raw 43 (Cache.raw.codes[43]!),
+     Translation.functionToTalos Cache.raw 44 (Cache.raw.codes[44]!),
+     Translation.functionToTalos Cache.raw 45 (Cache.raw.codes[45]!),
+     Translation.functionToTalos Cache.raw 46 (Cache.raw.codes[46]!)
+    ] =
+    [Project.EulerOutwardMaximum.func0Def, Project.EulerOutwardMaximum.func1Def, Project.EulerOutwardMaximum.func2Def, Project.EulerOutwardMaximum.func3Def, Project.EulerOutwardMaximum.func4Def, Project.EulerOutwardMaximum.func5Def, Project.EulerOutwardMaximum.func6Def, Project.EulerOutwardMaximum.func7Def, Project.EulerOutwardMaximum.func8Def, Project.EulerOutwardMaximum.func9Def, Project.EulerOutwardMaximum.func10Def, Project.EulerOutwardMaximum.func11Def, Project.EulerOutwardMaximum.func12Def, Project.EulerOutwardMaximum.func13Def, Project.EulerOutwardMaximum.func14Def, Project.EulerOutwardMaximum.func15Def, Project.EulerOutwardMaximum.func16Def, Project.EulerOutwardMaximum.func17Def, Project.EulerOutwardMaximum.func18Def, Project.EulerOutwardMaximum.func19Def, Project.EulerOutwardMaximum.func20Def, Project.EulerOutwardMaximum.func21Def, Project.EulerOutwardMaximum.func22Def, Project.EulerOutwardMaximum.func23Def, Project.EulerOutwardMaximum.func24Def, Project.EulerOutwardMaximum.func25Def, Project.EulerOutwardMaximum.func26Def, Project.EulerOutwardMaximum.func27Def, Project.EulerOutwardMaximum.func28Def, Project.EulerOutwardMaximum.func29Def, Project.EulerOutwardMaximum.func30Def, Project.EulerOutwardMaximum.func31Def, Project.EulerOutwardMaximum.func32Def, Project.EulerOutwardMaximum.func33Def, Project.EulerOutwardMaximum.func34Def, Project.EulerOutwardMaximum.func35Def, Project.EulerOutwardMaximum.func36Def, Project.EulerOutwardMaximum.func37Def, Project.EulerOutwardMaximum.func38Def, Project.EulerOutwardMaximum.func39Def, Project.EulerOutwardMaximum.func40Def, Project.EulerOutwardMaximum.func41Def, Project.EulerOutwardMaximum.func42Def, Project.EulerOutwardMaximum.func43Def, Project.EulerOutwardMaximum.func44Def, Project.EulerOutwardMaximum.func45Def, Project.EulerOutwardMaximum.func46Def]
+  rw [function0_eq, function1_eq, function2_eq, function3_eq, function4_eq, function5_eq, function6_eq, function7_eq, function8_eq, function9_eq, function10_eq, function11_eq, function12_eq, function13_eq, function14_eq, function15_eq, function16_eq, function17_eq, function18_eq, function19_eq, function20_eq, function21_eq, function22_eq, function23_eq, function24_eq, function25_eq, function26_eq, function27_eq, function28_eq, function29_eq, function30_eq, function31_eq, function32_eq, function33_eq, function34_eq, function35_eq, function36_eq, function37_eq, function38_eq, function39_eq, function40_eq, function41_eq, function42_eq, function43_eq, function44_eq, function45_eq, function46_eq]
+
+def executionCache : Wasm.Module :=
+  Project.EulerOutwardMaximum.«module»
+
+theorem translation_cache_eq :
+    Translation.module Cache.raw = executionCache := by
+  unfold Translation.module executionCache
+  rw [functions_eq]
+  rfl
+
+theorem artifact_correct_of (Property : Wasm.Module → Prop)
+    (behavior : Property executionCache) :
+    ∃ raw validated,
+      decode artifactBytes = .ok raw ∧
+      validate raw = .ok validated ∧
+      CoreValid raw ∧
+      Property validated.toTalos := by
+  rcases cache_validation_exists with ⟨validated, hvalidate⟩
+  have htranslation : validated.toTalos = executionCache := by
+    rw [ValidatedModule.toTalos, Proof.validate_raw_eq hvalidate,
+      translation_cache_eq]
+  refine ⟨Cache.raw, validated, decode_eq_cache, hvalidate,
+    Proof.validate_sound hvalidate, ?_⟩
+  rw [htranslation]
+  exact behavior
+
+theorem artifact_module_eq_cache :
+    ∃ raw validated,
+      decode artifactBytes = .ok raw ∧
+      validate raw = .ok validated ∧
+      CoreValid raw ∧
+      validated.toTalos = executionCache := by
+  exact artifact_correct_of (fun module_ => module_ = executionCache) rfl
+
+theorem artifact_interfaceUpper_exact :
+    ∃ raw validated,
+      decode artifactBytes = .ok raw ∧
+      validate raw = .ok validated ∧
+      CoreValid raw ∧
+      Spec.ExactSpecFor validated.toTalos := by
+  exact artifact_correct_of Spec.ExactSpecFor Spec.interfaceUpper_exact
+
+#print axioms artifact_interfaceUpper_exact
+
+theorem artifact_interfaceUpper_behavior :
+    ∃ raw validated,
+      decode artifactBytes = .ok raw ∧
+      validate raw = .ok validated ∧
+      CoreValid raw ∧
+      Spec.BehaviorSpecFor validated.toTalos := by
+  exact artifact_correct_of Spec.BehaviorSpecFor Spec.interfaceUpper_behavior
+
+#print axioms artifact_interfaceUpper_behavior
+end Project.EulerOutwardMaximum.Artifact
